GroupoidModel/Russell_PER_MS/GCongr.lean
@@ -3,7 +3,8 @@ import Mathlib.Tactic.GCongr
 
 /-! # `gcongr` lemmas
 
-In this module we prove special-case congruence lemmas for use with `gcongr`. -/
+In this module we prove special-case congruence lemmas for use with `gcongr`.
+Some of these have fewer premises than general congruences. -/
 
 /- Note: `refl` lemmas are not marked `@[refl]`
 because the `rfl` tactic expects unconditional reflexivity. -/
